Ported revisions 5727:5741 from HOL to HOL-Omega. This includes recent revisions to the prekernel (locations), rule inductive definitions, and the mc-logic example.

examples/ARM/v4/assemblerML.sig
@@ -1,5 +1,7 @@
 signature assemblerML =
 sig
+   val armErr          : TextIO.outstream ref
+
    val register2int   : Data.register -> int
    val int2register   : int -> Data.register
 
