src/IndDef/IndDefLib.sig
@@ -3,11 +3,11 @@ sig
   include Abbrev
   type monoset = InductiveDefinition.monoset
 
-  val term_of       : term quotation -> term
-  val term_of_absyn : Absyn.absyn -> term
+  val term_of       : term quotation -> term * locn.locn list
+  val term_of_absyn : Absyn.absyn -> term * locn.locn list
 
   val Hol_reln      : term quotation -> thm * thm * thm
-  val Hol_mono_reln : monoset -> term -> thm * thm * thm
+  val Hol_mono_reln : monoset -> (term * locn.locn list) -> thm * thm * thm
 
   val derive_mono_strong_induction : monoset -> thm * thm -> thm
   val derive_strong_induction : thm * thm -> thm
