examples/mc-logic/addressScript.sml
@@ -1,0 +1,353 @@
+
+open HolKernel boolLib bossLib Parse;
+open wordsTheory wordsLib bitTheory arithmeticTheory fcpTheory;
+
+val _ = new_theory "address";
+
+infix \\ << >>
+
+val op \\ = op THEN;
+val op << = op THENL;
+val op >> = op THEN1;
+
+val RW = REWRITE_RULE;
+val RW1 = ONCE_REWRITE_RULE;
+
+
+val aligned_def = Define `aligned (x:word32) = (x && 3w = 0w)`;
+
+val addr32_def = Define `addr32 (x:word30) = (w2w x << 2):word32`;
+val addr30_def = Define `addr30 (x:word32) = ((31 >< 2) x):word30`;
+
+val ZERO_word30 = store_thm("ZERO_word30",
+  ``1073741824w = 0w:word30``,
+  ONCE_REWRITE_TAC [GSYM n2w_mod] \\ SIMP_TAC (std_ss++SIZES_ss) []);
+
+val lower_addr32_ADD = store_thm("lower_addr32_ADD",
+  ``!w x. (1 >< 0) (addr32 x + w) = ((1 >< 0) w):word2``,
+  wordsLib.Cases_word
+  \\ REWRITE_TAC [addr32_def,EVAL ``dimindex (:32)``,w2w_def,word_lsl_n2w]
+  \\ EVAL_TAC \\ REWRITE_TAC [BITS_def,MOD_2EXP_def,DIV_2EXP_def]
+  \\ EVAL_TAC \\ REWRITE_TAC [DIV_1]
+  \\ REWRITE_TAC [(GSYM o EVAL) ``4 * 1073741824``]
+  \\ `0 < 4 /\ 0 < 1073741824` by EVAL_TAC
+  \\ ASM_SIMP_TAC bool_ss [MOD_MULT_MOD,MOD_MOD,MOD_TIMES]);
+
+val addr32_eq_0 = store_thm("addr32_eq_0",
+  ``!x. (1 >< 0) (addr32 x) = 0w:word2``,
+  ONCE_REWRITE_TAC [(GSYM o REWRITE_CONV [WORD_ADD_0]) ``addr32 x + 0w``]
+  \\ REWRITE_TAC [lower_addr32_ADD] \\ EVAL_TAC);
+
+val addr32_n2w = store_thm ("addr32_n2w", 
+  ``!n. (addr32 (n2w n)  = n2w (4 * n))``,
+  REWRITE_TAC [addr32_def, DECIDE ``2 = 1 + 1``, GSYM LSL_ADD, 
+               LSL_ONE,w2w_def, word_add_n2w, n2w_11, dimword_32]
+  \\ `!n. n + n + (n + n) = 4*n` by DECIDE_TAC
+  \\ ASM_SIMP_TAC std_ss [w2n_n2w, dimword_30, MOD_COMMON_FACTOR]);
+
+val n2w_and_1 = store_thm("n2w_and_1",
+  ``!n. (n2w n) && 1w = n2w (n MOD 2):'a word``,
+  REWRITE_TAC [CART_EQ] \\ ONCE_REWRITE_TAC [word_index_n2w]
+  \\ SIMP_TAC bool_ss [word_and_def,FCP_BETA] \\ REPEAT STRIP_TAC 
+  \\ ONCE_REWRITE_TAC [word_index_n2w] \\ ASM_REWRITE_TAC []
+  \\ Cases_on `i` THEN1 ASM_SIMP_TAC std_ss [BIT_def,BITS_THM2]
+  \\ REWRITE_TAC [BIT_def,BITS_THM,DECIDE ``SUC (SUC n) - SUC n = 1``]
+  \\ SIMP_TAC std_ss [GSYM DIV_DIV_DIV_MULT,ZERO_LT_EXP,EXP]
+  \\ SIMP_TAC std_ss [MOD_LESS,LESS_DIV_EQ_ZERO]);
+
+val n2w_and_3 = store_thm("n2w_and_3",
+  ``!n. (n2w n) && 3w = n2w (n MOD 4):'a word``,
+  REWRITE_TAC [CART_EQ] \\ ONCE_REWRITE_TAC [word_index_n2w]
+  \\ SIMP_TAC bool_ss [word_and_def,FCP_BETA] \\ REPEAT STRIP_TAC 
+  \\ ONCE_REWRITE_TAC [word_index_n2w] \\ ASM_REWRITE_TAC []
+  \\ `(i = 0) \/ (i = 1) \/ (2 <= i)` by DECIDE_TAC << [  
+    ASM_SIMP_TAC std_ss [BIT_def,BITS_THM2]
+    \\ SIMP_TAC bool_ss [GSYM (EVAL ``2*2``),MOD_MULT_MOD,EVAL ``0<2``],
+    ASM_SIMP_TAC std_ss [BIT_def,BITS_THM2],
+    REWRITE_TAC [BIT_def,BITS_THM,GSYM (EVAL ``2**2``)]
+    \\ `2**2 <= 2**i` by ASM_SIMP_TAC std_ss [EXP_BASE_LE_MONO]
+    \\ `n MOD (2**2) < 2**2` by ASM_SIMP_TAC std_ss [MOD_LESS]        
+    \\ `3 < 2**2` by EVAL_TAC
+    \\ IMP_RES_TAC LESS_LESS_EQ_TRANS
+    \\ ASM_SIMP_TAC bool_ss [LESS_DIV_EQ_ZERO,ZERO_MOD,ZERO_LT_TWOEXP,EVAL ``0 = 1``]]);
+
+val aligned_MULT = store_thm("aligned_MULT",
+  ``!x y. aligned x ==> aligned (x + 4w * y)``,
+  Cases_word \\ Cases_word
+  \\ REWRITE_TAC [word_add_n2w,word_mul_n2w,aligned_def,n2w_and_3]
+  \\ ONCE_REWRITE_TAC [ADD_COMM] \\ ONCE_REWRITE_TAC [MULT_COMM] 
+  \\ SIMP_TAC std_ss [MOD_TIMES]);
+
+val addr32_and_3w = store_thm("addr32_and_3w",
+  ``!x. (addr32 x) && 3w = 0w``,
+  wordsLib.Cases_word \\ REWRITE_TAC [addr32_n2w,n2w_and_3]
+  \\ SIMP_TAC std_ss [RW1 [MULT_COMM] MOD_EQ_0]);
+
+val aligned_addr32 = store_thm("aligned_addr32",
+  ``!x. aligned (addr32 x)``,
+  REWRITE_TAC [aligned_def,addr32_and_3w]);
+
+val addr30_n2w = store_thm("addr30_n2w",
+  ``!n. addr30 (n2w n) = n2w (n DIV 4)``,
+  REWRITE_TAC [addr30_def] \\ EVAL_TAC
+  \\ REWRITE_TAC [(GSYM o EVAL) ``1073741824 * 4``]
+  \\ `0 < 4 /\ 0 < 1073741824` by EVAL_TAC
+  \\ ASM_SIMP_TAC bool_ss [MOD_MULT_MOD,MOD_MOD,MOD_TIMES]
+  \\ REWRITE_TAC [BITS_def,MOD_2EXP_def,DIV_2EXP_def]
+  \\ EVAL_TAC \\ ASM_SIMP_TAC bool_ss [MOD_MOD]);
+
+val addr30_addr32_ADD = store_thm("addr30_addr32_ADD",
+  ``!x y. addr30 (addr32 x + y) = x + addr30 y``,
+  wordsLib.Cases_word \\ wordsLib.Cases_word
+  \\ REWRITE_TAC [addr30_n2w,addr32_n2w,word_add_n2w]
+  \\ SIMP_TAC std_ss [ONCE_REWRITE_RULE [MULT_COMM] ADD_DIV_ADD_DIV]);
+
+val addr30_addr32_LEMMA = prove(
+  ``!a. (addr30 (addr32 a + 0w) = a) /\ 
+        (addr30 (addr32 a + 1w) = a) /\ 
+        (addr30 (addr32 a + 2w) = a) /\ 
+        (addr30 (addr32 a + 3w) = a)``,
+  SIMP_TAC std_ss [addr30_addr32_ADD,addr30_n2w,WORD_ADD_0]);
+
+val addr30_addr32 = store_thm("addr30_addr32",
+  ``!x. (addr30 (addr32 x) = x) /\
+        (addr30 (addr32 x + 0w) = x) /\ 
+        (addr30 (addr32 x + 1w) = x) /\ 
+        (addr30 (addr32 x + 2w) = x) /\ 
+        (addr30 (addr32 x + 3w) = x)``,
+  REWRITE_TAC [REWRITE_RULE [WORD_ADD_0] addr30_addr32_LEMMA,addr30_addr32_LEMMA]);
+
+val EXISTS_addr30 = store_thm("EXISTS_addr30",
+  ``!x. (x && 3w = 0w) ==> ?y. x = addr32 y``,
+  wordsLib.Cases_word \\ REWRITE_TAC [n2w_and_3]  
+  \\ `4 < dimword (:32)` by EVAL_TAC
+  \\ `n MOD 4 < 4` by ASM_SIMP_TAC std_ss [MOD_LESS]
+  \\ `n MOD 4 < dimword (:32)` by DECIDE_TAC
+  \\ ASM_SIMP_TAC bool_ss [n2w_11,ZERO_LT_dimword,LESS_MOD]
+  \\ STRIP_TAC \\ Q.EXISTS_TAC `n2w (n DIV 4)`
+  \\ REWRITE_TAC [addr32_n2w] \\ ONCE_REWRITE_TAC [MULT_COMM]
+  \\ MATCH_MP_TAC (METIS_PROVE [] ``(x = y) ==> (f x = f y)``)
+  \\ CONV_TAC (RATOR_CONV (ONCE_REWRITE_CONV [MATCH_MP DIVISION (DECIDE ``0<4``)]))
+  \\ ASM_SIMP_TAC std_ss []);
+
+val add32_addr30 = store_thm("addr32_addr30",
+  ``!x. (x && 3w = 0w) ==> (addr32 (addr30 x) = x)``,
+  REPEAT STRIP_TAC \\ IMP_RES_TAC EXISTS_addr30 \\ ASM_REWRITE_TAC [addr30_addr32]);
+
+val addr32_ADD = store_thm ("addr32_ADD", 
+  ``!v w. (addr32 (v + w)  = addr32 v + addr32 w)``,
+  Cases_word \\ Cases_word
+  \\ REWRITE_TAC [addr32_n2w,word_add_n2w,LEFT_ADD_DISTRIB]);
+
+val addr32_NEG = store_thm("addr32_NEG",
+  ``!w. addr32 ($- w) = $- (addr32 w)``,
+  wordsLib.Cases_word \\ REWRITE_TAC [addr32_n2w] 
+  \\ wordsLib.WORDS_TAC \\ REWRITE_TAC [addr32_n2w]
+  \\ SIMP_TAC (std_ss++wordsLib.SIZES_ss) [n2w_11,LEFT_SUB_DISTRIB,MOD_COMMON_FACTOR]);
+
+val addr32_SUB = store_thm ("addr32_SUB", 
+  ``!v w. (addr32 (v - w)  = addr32 v - addr32 w)``,
+  REWRITE_TAC [word_sub_def,addr32_ADD,addr32_NEG]);
+  
+val addr32_SUC = store_thm("addr32_SUC",
+  ``!p. addr32 (p + 1w) = addr32 p + 4w``,
+  SIMP_TAC std_ss [addr32_ADD,addr32_n2w]);
+
+val addr30_ADD = store_thm("addr30_ADD",
+  ``!x m. addr30 x + n2w m = addr30 (x + n2w (4 * m))``,
+  Cases_word \\ REWRITE_TAC [addr30_n2w,word_add_n2w]
+  \\ ONCE_REWRITE_TAC [ADD_COMM]
+  \\ SIMP_TAC std_ss [GSYM ADD_DIV_ADD_DIV,AC MULT_COMM MULT_ASSOC]);  
+
+val ADD_LSL = store_thm("ADD_LSL",
+  ``!v w n. (v + w) << n = (v << n) + (w << n)``,
+  Induct_on `n` \\ SIMP_TAC std_ss [SHIFT_ZERO,SUC_ONE_ADD,GSYM LSL_ADD,LSL_ONE]
+  \\ METIS_TAC [WORD_ADD_ASSOC,WORD_ADD_COMM]);
+
+val addr32_11 = store_thm("addr32_11",
+  ``!a b. ((addr32 a = addr32 b) = (a = b)) /\ 
+          ((addr32 a = addr32 b + 0w) = (a = b)) /\ 
+          ((addr32 a + 0w = addr32 b) = (a = b)) /\ 
+          ((addr32 a + 0w = addr32 b + 0w) = (a = b)) /\ 
+          ((addr32 a + 1w = addr32 b + 1w) = (a = b)) /\ 
+          ((addr32 a + 2w = addr32 b + 2w) = (a = b)) /\ 
+          ((addr32 a + 3w = addr32 b + 3w) = (a = b))``,
+  wordsLib.Cases_word \\ wordsLib.Cases_word 
+  \\ REWRITE_TAC [WORD_EQ_ADD_RCANCEL,WORD_ADD_0]
+  \\ FULL_SIMP_TAC (std_ss++wordsLib.SIZES_ss) [addr32_n2w,n2w_11]
+  \\ `4 * n < 4294967296 /\ 4 * n' < 4294967296` by DECIDE_TAC
+  \\ ASM_SIMP_TAC std_ss [LESS_MOD,EQ_MULT_LCANCEL]);
+
+val addr32_EQ_0 = store_thm("addr32_EQ_0",
+  ``!a. (addr32 a = 0w) = (a = 0w)``,
+  REWRITE_TAC [SIMP_RULE std_ss [addr32_n2w] (Q.SPECL [`a`,`0w`] addr32_11)]);
+
+val addr32_NEQ_addr32_LEMMA = prove(
+  ``!a b. ~(addr32 a = addr32 b + 1w) /\ 
+          ~(addr32 a = addr32 b + 2w) /\ 
+          ~(addr32 a = addr32 b + 3w) /\ 
+          ~(addr32 a + 1w = addr32 b + 2w) /\ 
+          ~(addr32 a + 1w = addr32 b + 3w) /\ 
+          ~(addr32 a + 2w = addr32 b + 3w)``,
+  wordsLib.Cases_word \\ wordsLib.Cases_word
+  \\ FULL_SIMP_TAC (std_ss++wordsLib.SIZES_ss) [addr32_n2w,word_add_n2w,n2w_11]
+  \\ REWRITE_TAC [GSYM (EVAL ``4 * 1073741824``)]
+  \\ `0 < 4 /\ 0 < 1073741824` by EVAL_TAC
+  \\ `4 * n' + 1 < 4 * 1073741824` by DECIDE_TAC
+  \\ `4 * n' + 2 < 4 * 1073741824` by DECIDE_TAC
+  \\ `4 * n' + 3 < 4 * 1073741824` by DECIDE_TAC
+  \\ `4 * n + 1 < 4 * 1073741824` by DECIDE_TAC
+  \\ `4 * n + 2 < 4 * 1073741824` by DECIDE_TAC
+  \\ ASM_SIMP_TAC bool_ss [GSYM MOD_COMMON_FACTOR,LESS_MOD]
+  \\ ONCE_REWRITE_TAC [MULT_SYM]
+  \\ `!k. (k * 4) MOD 4 = 0` by SIMP_TAC std_ss [MOD_EQ_0]
+  \\ `!k. (k * 4 + 1) MOD 4 = 1` by SIMP_TAC std_ss [MOD_MULT]
+  \\ `!k. (k * 4 + 2) MOD 4 = 2` by SIMP_TAC std_ss [MOD_MULT]
+  \\ `!k. (k * 4 + 3) MOD 4 = 3` by SIMP_TAC std_ss [MOD_MULT]
+  \\ METIS_TAC [EVAL ``0 = 1``,EVAL ``0 = 2``,EVAL ``0 = 3``,
+                EVAL ``1 = 2``,EVAL ``1 = 3``,EVAL ``2 = 3``]);
+
+val addr32_NEQ_addr32 = store_thm("addr32_NEQ_addr32",
+  ``!a b. ~(addr32 a + 0w = addr32 b + 1w) /\ 
+          ~(addr32 a + 0w = addr32 b + 2w) /\ 
+          ~(addr32 a + 0w = addr32 b + 3w) /\ 
+          ~(addr32 a + 1w = addr32 b + 2w) /\ 
+          ~(addr32 a + 1w = addr32 b + 3w) /\ 
+          ~(addr32 a + 2w = addr32 b + 3w) /\
+          ~(addr32 a + 1w = addr32 b + 0w) /\ 
+          ~(addr32 a + 2w = addr32 b + 0w) /\ 
+          ~(addr32 a + 3w = addr32 b + 0w) /\ 
+          ~(addr32 a + 2w = addr32 b + 1w) /\ 
+          ~(addr32 a + 3w = addr32 b + 1w) /\ 
+          ~(addr32 a + 3w = addr32 b + 2w) /\ 
+          ~(addr32 a + 1w = addr32 b) /\ 
+          ~(addr32 a + 2w = addr32 b) /\ 
+          ~(addr32 a + 3w = addr32 b) /\
+          ~(addr32 a = addr32 b + 1w) /\ 
+          ~(addr32 a = addr32 b + 2w) /\ 
+          ~(addr32 a = addr32 b + 3w)``, 
+  REWRITE_TAC [WORD_ADD_0,addr32_NEQ_addr32_LEMMA,GSYM addr32_NEQ_addr32_LEMMA]);  
+
+val EXISTS_addr32 = store_thm("EXISTS_addr32",
+  ``!p. ?a. (p = addr32 a + 0w) \/ (p = addr32 a + 1w) \/ 
+            (p = addr32 a + 2w) \/ (p = addr32 a + 3w)``,
+  wordsLib.Cases_word
+  \\ STRIP_ASSUME_TAC (REWRITE_RULE [EVAL ``0 < 4``] (Q.SPECL [`n`,`4`] DA))
+  \\ ASM_REWRITE_TAC [] \\ Q.EXISTS_TAC `n2w q` \\ REWRITE_TAC [addr32_n2w,word_add_n2w]
+  \\ ONCE_REWRITE_TAC [DECIDE ``4 * n = n * 4``]
+  \\ Cases_on `r` \\ ASM_REWRITE_TAC []
+  \\ Cases_on `n'` \\ ASM_REWRITE_TAC [EVAL ``SUC 0``]
+  \\ Cases_on `n''` \\ ASM_REWRITE_TAC [EVAL ``SUC (SUC 0)``]
+  \\ Cases_on `n'` \\ ASM_REWRITE_TAC [EVAL ``SUC (SUC (SUC 0))``]
+  \\ FULL_SIMP_TAC std_ss [ADD1,GSYM ADD_ASSOC]
+  \\ `n'' < 0` by DECIDE_TAC \\ FULL_SIMP_TAC bool_ss [EVAL ``n < 0``]);
+
+val addr32_ABSORB_CONST = store_thm("addr32_ABSORB_CONST",
+  ``(addr32 x + 0w  = addr32 x) /\ 
+    (addr32 x + 4w  = addr32 (x + 1w)) /\ 
+    (addr32 x + 8w  = addr32 (x + 2w)) /\ 
+    (addr32 x + 12w = addr32 (x + 3w)) /\ 
+    (addr32 x + 16w = addr32 (x + 4w)) /\ 
+    (addr32 x + 20w = addr32 (x + 5w)) /\
+    (addr32 x + 24w = addr32 (x + 6w)) /\
+    (addr32 x + 28w = addr32 (x + 7w)) /\
+    (addr32 x + 32w = addr32 (x + 8w)) /\
+    (addr32 x + 36w = addr32 (x + 9w)) /\
+    (addr32 x + 40w = addr32 (x + 10w)) /\
+    (addr32 x - 0w  = addr32 (x - 0w)) /\
+    (addr32 x - 4w  = addr32 (x - 1w)) /\ 
+    (addr32 x - 8w  = addr32 (x - 2w)) /\ 
+    (addr32 x - 12w = addr32 (x - 3w)) /\ 
+    (addr32 x - 16w = addr32 (x - 4w)) /\ 
+    (addr32 x - 20w = addr32 (x - 5w)) /\
+    (addr32 x - 24w = addr32 (x - 6w)) /\
+    (addr32 x - 28w = addr32 (x - 7w)) /\
+    (addr32 x - 32w = addr32 (x - 8w)) /\
+    (addr32 x - 36w = addr32 (x - 9w)) /\
+    (addr32 x - 40w = addr32 (x - 10w))``,    
+  SIMP_TAC std_ss [addr32_ADD,addr32_SUB,addr32_n2w,WORD_ADD_0]);
+
+val ADDRESS_ROTATE = store_thm("ADDRESS_ROTATE",
+  ``!q:word32 z:word30. q #>> (8 * w2n ((1 >< 0) (addr32 z):word2)) = q``,
+  SIMP_TAC std_ss [addr32_eq_0,EVAL ``w2n (0w:word2)``] \\ STRIP_TAC \\ EVAL_TAC);
+
+val addr30_THM = store_thm("addr30_THM",
+  ``!x. addr30 x = n2w (w2n x DIV 4)``,
+  Cases_word \\ ASM_SIMP_TAC bool_ss [w2n_n2w,LESS_MOD,addr30_n2w]);
+
+val addr32_THM = store_thm("addr32_THM",
+  ``!x. addr32 x = n2w (4 * w2n x)``,
+  Cases_word \\ ASM_SIMP_TAC bool_ss [w2n_n2w,LESS_MOD,addr32_n2w]);
+
+val aligned_THM = store_thm("aligned_THM",
+  ``!p. aligned p = ?k. p = k * 4w``,
+  Cases_word \\ EQ_TAC \\ REPEAT STRIP_TAC
+  \\ FULL_SIMP_TAC bool_ss [n2w_and_3,aligned_def] << [
+    ASSUME_TAC (Q.SPEC `n` (MATCH_MP DIVISION (DECIDE ``0 < 4``)))
+    \\ REPEAT STRIP_TAC \\ ONCE_ASM_REWRITE_TAC []
+    \\ REWRITE_TAC [GSYM word_add_n2w,GSYM word_mul_n2w]
+    \\ Q.PAT_ASSUM `b /\ c` (fn th => ALL_TAC)
+    \\ ASM_REWRITE_TAC [WORD_ADD_0] \\ METIS_TAC [],
+    Q.UNDISCH_TAC `n2w n = k * 4w`
+    \\ Q.SPEC_TAC (`k`,`k`) \\ Cases_word
+    \\ ASM_SIMP_TAC bool_ss [word_mul_n2w,n2w_11,LESS_MOD]
+    \\ REWRITE_TAC [EVAL ``dimword (:32)``]
+    \\ REWRITE_TAC [GSYM (EVAL ``4 * 1073741824``)]
+    \\ SIMP_TAC bool_ss 
+        [MOD_MULT_MOD,DECIDE ``0 < 1073741824``,DECIDE ``0<4``,MOD_EQ_0]]);
+
+val aligned_and_1 = store_thm("aligned_and_1",
+  ``!x. aligned x ==> (x && 1w = 0w)``,        
+  REWRITE_TAC [aligned_THM] \\ NTAC 2 STRIP_TAC
+  \\ ASM_REWRITE_TAC [] \\ POP_ASSUM (fn th => ALL_TAC)
+  \\ Q.SPEC_TAC (`k`,`k`) \\ Cases
+  \\ REWRITE_TAC [word_mul_n2w,word_add_n2w,n2w_and_1,n2w_11]
+  \\ REWRITE_TAC [GSYM (EVAL ``2*2``),MULT_ASSOC]
+  \\ SIMP_TAC (std_ss++SIZES_ss) [MOD_EQ_0]);
+
+val aligned_add_1_and_1 = store_thm("aligned_add_1_and_1",
+  ``!x. aligned x ==> ~(x + 1w && 1w = 0w)``,        
+  REWRITE_TAC [aligned_THM] \\ NTAC 2 STRIP_TAC
+  \\ ASM_REWRITE_TAC [] \\ POP_ASSUM (fn th => ALL_TAC)
+  \\ Q.SPEC_TAC (`k`,`k`) \\ Cases
+  \\ REWRITE_TAC [word_mul_n2w,word_add_n2w,n2w_and_1,n2w_11]
+  \\ REWRITE_TAC [GSYM (EVAL ``2*2``),MULT_ASSOC]
+  \\ SIMP_TAC (std_ss++SIZES_ss) [MOD_TIMES]);
+
+val aligned_ADD = store_thm("aligned_ADD",
+  ``!x y. aligned x /\ aligned y ==> aligned (x + y)``,
+  REWRITE_TAC [aligned_THM] \\ REPEAT STRIP_TAC
+  \\ ASM_REWRITE_TAC [GSYM WORD_RIGHT_ADD_DISTRIB] \\ METIS_TAC []);
+  
+val word_arith_lemma1 = store_thm("word_arith_lemma1",
+  ``!n m. (n2w n + n2w m = n2w (n + m):'a word) /\
+          (x + n2w n + n2w m = x + n2w (n + m):'a word) /\
+          (x - n2w n - n2w m = x - n2w (n + m):'a word)``,
+  REWRITE_TAC [GSYM WORD_SUB_PLUS,word_add_n2w,GSYM WORD_ADD_ASSOC]);
+
+val word_arith_lemma2 = store_thm("word_arith_lemma2",
+  ``!n m. n2w n - (n2w m) :'a word = if n < m then $- (n2w (m-n)) else n2w (n-m)``,
+  REPEAT STRIP_TAC \\ Cases_on `n < m` \\ ASM_REWRITE_TAC []
+  \\ FULL_SIMP_TAC bool_ss [NOT_LESS,LESS_EQ]
+  \\ FULL_SIMP_TAC bool_ss [LESS_EQ_EXISTS,ADD1,DECIDE ``n+1+p-n = 1+p:num``]
+  \\ REWRITE_TAC [GSYM word_add_n2w,WORD_SUB_PLUS,WORD_SUB_REFL] 
+  \\ REWRITE_TAC [GSYM WORD_SUB_PLUS] 
+  \\ REWRITE_TAC [word_sub_def,WORD_ADD_0,DECIDE ``m+p-m=p:num``]
+  \\ REWRITE_TAC [GSYM WORD_ADD_ASSOC] \\ ONCE_REWRITE_TAC [WORD_ADD_COMM]
+  \\ REWRITE_TAC [GSYM word_sub_def,WORD_SUB_ADD]);
+  
+val word_arith_lemma3 = store_thm("word_arith_lemma3",
+  ``!x n m. x - n2w m + n2w n :'a word = if n < m then x - (n2w (m-n)) else x + n2w (n-m)``,
+  REWRITE_TAC [word_sub_def,GSYM WORD_ADD_ASSOC]
+  \\ REWRITE_TAC [GSYM (RW1 [WORD_ADD_COMM] word_sub_def),word_arith_lemma2] 
+  \\ REPEAT STRIP_TAC \\ Cases_on `n<m` \\ ASM_REWRITE_TAC []);
+
+val word_arith_lemma4 = store_thm("word_arith_lemma4",
+  ``!x n m. x + n2w n - n2w m :'a word = if n < m then x - (n2w (m-n)) else x + n2w (n-m)``,
+  REWRITE_TAC [word_sub_def,GSYM WORD_ADD_ASSOC]
+  \\ REWRITE_TAC [GSYM word_sub_def,word_arith_lemma2]
+  \\ REPEAT STRIP_TAC \\ Cases_on `n<m` \\ ASM_REWRITE_TAC [word_sub_def]);
+
+
+
+val _ = export_theory();
